create GarageDoor.v

src/Bedrock/End2End/X25519/MontgomeryLadder.v
@@ -19,7 +19,6 @@ Require Import Crypto.Bedrock.End2End.X25519.Field25519.
 Local Open Scope string_scope.
 Import ListNotations.
 
-
 Local Instance frep25519 : Field.FieldRepresentation(field_parameters:=field_parameters) := field_representation n Field25519.s c.
 Derive ladderstep SuchThat (ladderstep = ladderstep_body) As ladderstep_defn.
 Proof. vm_compute. subst; exact eq_refl. Qed.
@@ -49,14 +48,14 @@ Definition x25519_base : func := ("x25519_base", (["out"; "sk"], [], bedrock_fun
 Import LittleEndianList.
 Local Coercion F.to_Z : F >-> Z.
 Require Import bedrock2.WeakestPrecondition bedrock2.Semantics bedrock2.ProgramLogic.
-Require Import bedrock2.BasicC32Semantics bedrock2.Syntax bedrock2.Map.SeparationLogic.
+Require Import bedrock2.Syntax bedrock2.Map.SeparationLogic.
 Require Import coqutil.Map.OfListWord Coq.Init.Byte coqutil.Byte.
 Import ProgramLogic.Coercions.
 Local Notation "m =* P" := ((P%sep) m) (at level 70, only parsing) (* experiment*).
 Local Notation "xs $@ a" := (Array.array ptsto (word.of_Z 1) a xs) (at level 10, format "xs $@ a").
 Definition x25519_gallina := montladder_gallina (Field.M_pos(FieldParameters:=field_parameters)) Field.a24 (Z.to_nat (Z.log2 (Z.pos order))).
 Global Instance spec_of_x25519 : spec_of x25519 :=
-  fnspec! "x25519" out sk pk / (o s p : list Byte.byte) (R : mem -> Prop),
+  fnspec! "x25519" out sk pk / (o s p : list Byte.byte) (R : _ -> Prop),
   { requires t m := m =* s$@sk * p$@pk * o$@out * R /\
       length s = 32%nat /\ length p = 32%nat /\ length o = 32%nat /\ byte.unsigned (nth 31 p x00) <= 0x7f;
     ensures t' m := t=t' /\ m=* s$@sk ⋆ p$@pk ⋆ R ⋆
@@ -66,6 +65,11 @@ Local Instance spec_of_fe25519_from_word : spec_of "fe25519_from_word" := Field.
 Local Instance spec_of_fe25519_from_bytes : spec_of "fe25519_from_bytes" := Field.spec_of_from_bytes.
 Local Instance spec_of_fe25519_to_bytes : spec_of "fe25519_to_bytes" := Field.spec_of_to_bytes.
 Local Instance spec_of_montladder : spec_of "montladder" := spec_of_montladder(Z.to_nat (Z.log2 Curve25519.order)).
+
+Local Arguments word.rep : simpl never.
+Local Arguments word.wrap : simpl never.
+Local Arguments word.unsigned : simpl never.
+Local Arguments word.of_Z : simpl never.
 Lemma x25519_ok : program_logic_goal_for_function! x25519.
 Proof.
   repeat straightline.
@@ -73,11 +77,11 @@ Proof.
 
   straightline_call; ssplit.
   { eexists. ecancel_assumption. }
-  { unfold Field.FElem.
+  { cbv [Field.FElem].
     use_sep_assumption. cancel. cancel_seps_at_indices 0%nat 0%nat; cbn; trivial. eapply RelationClasses.reflexivity. }
   { unfold Field.bytes_in_bounds, frep25519, field_representation, Signature.field_representation, Representation.frep.
     match goal with |- ?P ?x ?z => let y := eval cbv in x in change (P y z) end; cbn.
-    repeat (destruct p as [|? p]; try (cbn in *;discriminate); []).
+    repeat (destruct p as [|? p]; try (cbn [length] in *;discriminate); []).
     cbn; cbn [nth] in *.
     cbv [COperationSpecifications.list_Z_bounded_by FoldBool.fold_andb_map map seq]; cbn.
     pose proof byte.unsigned_range as HH. setoid_rewrite <-Le.Z.le_sub_1_iff in HH. cbn in HH.
@@ -100,7 +104,7 @@ Proof.
   { rewrite H3. vm_compute. inversion 1. }
   repeat straightline.
 
-  unfold FElem in H22. extract_ex1_and_emp_in H22.
+  cbv [FElem] in H22. extract_ex1_and_emp_in H22.
   straightline_call; ssplit.
   { ecancel_assumption. }
   { transitivity 32%nat; auto. }
@@ -120,7 +124,7 @@ Proof.
 Qed.
 
 Global Instance spec_of_x25519_base : spec_of x25519_base :=
-  fnspec! "x25519_base" out sk / (o s : list Byte.byte) (R : mem -> Prop),
+  fnspec! "x25519_base" out sk / (o s : list Byte.byte) (R : _ -> Prop),
   { requires t m := m =* s$@sk * o$@out * R /\
       length s = 32%nat /\ length o = 32%nat;
     ensures t' m := t=t' /\ m=* s$@sk ⋆ R ⋆
@@ -165,139 +169,26 @@ Proof.
   use_sep_assumption; cancel. eapply RelationClasses.reflexivity.
 Qed.
 
-Require Import bedrock2Examples.LAN9250.
-Require Import bedrock2Examples.lightbulb.
-Require Import bedrock2Examples.chacha20.
-Require Import bedrock2Examples.memequal.
-Require Import bedrock2Examples.memswap.
-Require Import bedrock2Examples.memconst.
-Require Import Rupicola.Examples.Net.IPChecksum.IPChecksum.
-
-Import Coq.Init.Byte.
-Definition garageowner : list byte :=
-  [x7b; x06; x18; x0c; x54; x0c; xca; x9f; xa3; x16; x0b; x2f; x2b; x69; x89; x63; x77; x4c; xc1; xef; xdc; x04; x91; x46; x76; x8b; xb2; xbf; x43; x0e; x34; x34].
-
-Import Syntax.Coercions.
-
-Definition st : expr := 0x8000000.
-Definition pk : expr := 0x8000040.
-Definition buf : expr := 0x8000060.
-
-Definition init : func :=
-  ("init", ([], [], bedrock_func_body:(
-    $(memconst "pk" garageowner)($pk);
-    output! MMIOWRITE($0x10012038, $(Z.lor (Z.shiftl (0xf) 2) (Z.shiftl 1 9)));
-    output! MMIOWRITE($0x10012008, $(Z.lor (Z.shiftl 1 11) (Z.shiftl 1 12)));
-    output! MMIOWRITE($0x10024010, $2);
-    unpack! err = lan9250_init()
-  ))).
-
-Definition loop : func := ("loop", ([], [], bedrock_func_body:(
-  st=$st; pk=$pk; buf=$buf;
-  unpack! l, err = recvEthernet(buf);
-  require !err;
-  require ($63 < l);
-
-  ethertype = (((load1(buf + $12))&$0xff) << $8) | ((load1(buf + $13))&$0xff);
-  require ($(1536 - 1) < ethertype);
-  protocol = (load1(buf+$23))&$0xff;
-  require (protocol == $0x11);
-
-  if $(14+20+8 +2+32 +4) == l { (* getpk *)
-    memswap(buf, buf+$6, $6); (* ethernet address *)
-    memswap(buf+$(14+12), buf+$(14+16), $4); (* IP address *)
-    memswap(buf+$(14+20+0), buf+$(14+20+2), $2); (* UDP port *)
-    store1(buf+$(14+2), $0); (* ip length *)
-    store1(buf+$(14+3), $(20+ 8+ 32+2)); (* ip length *)
-    store1(buf+$(14+10), $0); (* preliminary ip checksum *)
-    store1(buf+$(14+11), $0); (* preliminary ip checksum *)
-
-    unpack! chk = ip_checksum(buf+$14, $20);
-    store1(buf+$(14+11), chk>>$8);
-    store1(buf+$(14+10), chk);
-
-    store1(buf+$(14+20+4), $0); (* udp length *)
-    store1(buf+$(14+20+5), $(8+ 32+2)); (* udp length *)
-    store1(buf+$(14+20+6), $0); (* udp checksum *)
-    store1(buf+$(14+20+7), $0); (* udp checksum *)
-
-    x25519_base(buf+$(14+20+8 +2), st+$32);
-    lan9250_tx(buf, $(14+20+8 +2+32))
-  } else if $(14+20+8 +2+16 +4) == l { (* operate *)
-    stackalloc 32 as tmp;
-    x25519(tmp, st+$32, pk);
-    unpack! set0 = memequal(tmp, buf+$(14+20+8 +2), $16);
-    unpack! set1 = memequal(tmp+$16, buf+$(14+20+8 +2), $16);
-
-    io! mmio_val = MMIOREAD($0x1001200c);
-    mmio_val = mmio_val & coq:(Z.clearbit (Z.clearbit (2^32-1) 11) 12);
-    output! MMIOWRITE($0x1001200c, mmio_val | (set1<<$1 | set0) << $11);
-
-    if (set0|set1) { (* rekey *)
-        chacha20_block(st, st, (*nonce*)pk, $0) (* NOTE: another impl? *)
-    }
-  }
-))).
+Require Import coqutil.Word.Naive.
 
 Definition funcs : list func :=
-  [ init;
-    loop; memswap; memequal; x25519; x25519_base; lan9250_tx;
-    memconst "pk" garageowner;
-
+  [ x25519; x25519_base;
     montladder;
     fe25519_to_bytes;
     fe25519_from_bytes;
     fe25519_from_word;
-    CSwap.cswap_body(word:=BasicC32Semantics.word)(field_parameters:=field_parameters)(field_representaton:=field_representation n s c);
+    CSwap.cswap_body(word:=word32)(field_parameters:=field_parameters)(field_representaton:=field_representation n s c);
     fe25519_copy;
-    fe25519_inv(word:=BasicC32Semantics.word)(field_parameters:=field_parameters);
+    fe25519_inv(word:=word32)(field_parameters:=field_parameters);
     ladderstep;
     fe25519_mul;
     fe25519_add;
     fe25519_sub;
     fe25519_square;
-    fe25519_scmula24 ]
-    ++ lightbulb.function_impls
-    ++ [chacha20_quarter; chacha20_block]
-    ++ [ip_checksum_br2fn].
+    fe25519_scmula24 ].
 
 
 Definition montladder_c_module := ToCString.c_module funcs.
-
-Require compiler.ToplevelLoop.
-Definition ml: MemoryLayout.MemoryLayout(word:=BasicC32Semantics.word) := {|
-  MemoryLayout.code_start    := word.of_Z 0x20400000;
-  MemoryLayout.code_pastend  := word.of_Z 0x21400000;
-  MemoryLayout.heap_start    := word.of_Z 0x80000000;
-  MemoryLayout.heap_pastend  := word.of_Z 0x80002000;
-  MemoryLayout.stack_start   := word.of_Z 0x80002000;
-  MemoryLayout.stack_pastend := word.of_Z 0x80004000;
-|}.
-
-
-
-Derive garagedoor_compiler_result SuchThat
-  (ToplevelLoop.compile_prog (string_keyed_map:=@SortedListString.map) MMIO.compile_ext_call ml funcs
-  = Success garagedoor_compiler_result)
-  As garagedoor_compiler_result_ok.
-Proof.
-  match goal with x := _ |- _ => cbv delta [x]; clear x end.
-  vm_compute.
-  match goal with |- @Success ?A ?x = Success ?e => is_evar e;
-    exact (@eq_refl (result A) (@Success A x)) end.
-Qed.
-
-Set Printing Implicit.
-Definition garagedoor_stack_size := snd garagedoor_compiler_result.
-Definition garagedoor_finfo := snd (fst garagedoor_compiler_result).
-Definition garagedoor_insns := fst (fst garagedoor_compiler_result).
-Definition garagedoor_bytes := Pipeline.instrencode garagedoor_insns.
-Definition garagedoor_symbols : list byte := Symbols.symbols garagedoor_finfo.
-
-(*
-Compute garagedoor_finfo.
-Compute ToCString.c_func fe25519_to_bytes. (* contains big constants that are used many times, could save some instructions by assigning them to a variable, otherwise it requires two instructions (instead of 0) each time the constant is reused *)
-*)
 
 Derive montladder_compiler_result SuchThat
        (compile
@@ -326,5 +217,5 @@ Module PrintAssembly.
   Unset Printing Coercions.
 
   (* Compute garagedoor_finfo. (* fe25519_mul is more than 10KB in just one function *) *)
-  Goal True. let r := eval cbv in garagedoor_insns in idtac (* r *). Abort.
+  Goal True. let r := eval cbv in montladder_insns in idtac (* r *). Abort.
 End PrintAssembly.
